major refactor on Coq naming, bisimulation, minor fix in model generation

CACoq/CaMain.v
@@ -4,7 +4,22 @@ Require Import Classes.EquivDec.
 Require Import Coq.Program.Program.
 Require Import QArith.
 Require Import Coq.Numbers.BinNums.
+Require Import Coq.micromega.Lia.
 
+Open Scope Q_scope.
+
+(* The following lemma was formalized thanks to anonymous reviewers' contribution *)
+Lemma orderZofNat : forall n, forall a, (Z.of_nat (S n) + a) # 1 < Z.of_nat (S (S n)) + a # 1.
+Proof.
+intros.
+assert (forall z, z # 1 < (z + 1) # 1).
++ intros. assert (inject_Z z < inject_Z (z + 1)). rewrite <- Zlt_Qlt. 
+  omega. unfold inject_Z in H. exact H.
++ assert (forall b, forall a, (b + a) # 1 < ((b + 1) + a) # 1).
+  intros. rewrite <- Z.add_assoc. rewrite (Z.add_comm 1).
+  rewrite Z.add_assoc. apply H.
+  assert (forall n, Z.of_nat (S n) = ((Z.of_nat n) + 1)%Z).
+  intro. simpl. lia. rewrite (H1 ((S n))). apply H0. Defined.
 
 Close Scope Q_scope.
 
@@ -31,6 +46,19 @@ Proof.
 all:congruence.
 Defined.
 
+Instance pair_eqdec A B `(EqDec A eq) `(EqDec B eq) : EqDec (A * B) eq :=
+{
+  equiv_dec x y:=
+    match x, y with
+      | (a, b), (c,d) => if a == c then
+                            if b == d then in_left else in_right
+                         else in_right
+    end
+}.
+Proof.
+all: congruence.
+Defined.
+
 Program Fixpoint s1_in_s2 {A} `{EqDec A eq} (s1 s2 : set A) :=
   match s1 with
     | [] => true
@@ -39,8 +67,8 @@ Program Fixpoint s1_in_s2 {A} `{EqDec A eq} (s1 s2 : set A) :=
 
 Fixpoint set_eq {A} `{EqDec A eq} (s1 s2 : set A) :=
   if (length s1 == length s2) then
-      if (s1_in_s2 s1 s2 == true) then
-          if (s1_in_s2 s2 s1 == true) then true else false
+      if (s1_in_s2 s1 s2) then
+          if (s1_in_s2 s2 s1) then true else false
       else false
   else false.
 
@@ -51,15 +79,19 @@ Lemma set_eq_sound {A} `{EqDec A eq} : forall s1 : set A, forall s2 : set A,
   split.
   - intros. destruct s1. destruct s2.
   + split. reflexivity. split. assumption. assumption.
-  + inversion H0. 
-  + unfold set_eq in H0. destruct equiv_dec in H0. destruct equiv_dec in H0. destruct equiv_dec in H0.
-    auto. inversion H0. inversion H0. inversion H0.
+  + inversion H0.
+  + unfold set_eq in H0. destruct equiv_dec in H0.
+    case_eq (s1_in_s2 (a :: s1) s2). case_eq (s1_in_s2 s2 (a :: s1)). intros. rewrite H1 in H0. rewrite H2 in H0. inversion e.
+    split. reflexivity. auto. intros. rewrite H2 in H0. rewrite H1 in H0. inversion H0. intros. 
+    rewrite H1 in H0. inversion H0. congruence. 
   - intros. destruct s1. destruct s2.
   + reflexivity.
   + destruct H0. inversion H0.
   + simpl. destruct H0. destruct H1. simpl in H0. rewrite H0.
     simpl s1_in_s2 in H1. rewrite H1. rewrite H2. repeat simpl. destruct equiv_dec. reflexivity. congruence.
   Defined.
+
+
 (* --------------------------------------------------------------------------------------------------------------- *)
 
 Module ConstraintAutomata.
@@ -67,83 +99,83 @@ Module ConstraintAutomata.
 
     Variable state name data: Set. 
 
-    Context `{EqDec name eq} `{EqDec state eq} `{EqDec (option data) eq}.
+    Context `{EqDec name eq} `{EqDec state eq} `{EqDec (data) eq}.
 
-    Notation " a <? b " :=  (negb (Qle_bool b a)).
+    Notation " a <? b " := (negb (Qle_bool b a)).
     Notation "a =? b" := (Qeq_bool a b).
 
-    Record port := mkport{
+    Record tds := mktds {
       id : name;
-      dataAssignment : nat -> option data; 
+      dataAssignment : nat -> data; 
       timeStamp : nat -> QArith_base.Q;
-      portCond : forall n:nat, Qlt (timeStamp n) (timeStamp (S n));
+      tdsCond : forall n:nat, Qlt (timeStamp n) (timeStamp (S n));
       index : nat
 
     }.
 
-    Inductive DC := 
-    | tDc : DC 
-    | dc : name -> option data -> DC 
-    | eqDc : name -> name -> DC
-    | andDc : DC -> DC -> DC
-    | orDc  : DC -> DC -> DC
-    | trDc  : (option data -> option data) -> name -> name -> DC 
-    | negDc : DC -> DC.
-
-    Check DC.
+    Inductive DC name data:= 
+    | tDc : DC name data
+    | dc : name -> data -> DC name data
+    | eqDc : name -> name -> DC name data
+    | andDc : DC name data -> DC name data -> DC name data
+    | orDc  : DC name data -> DC name data -> DC name data
+    | trDc  : (data -> data) -> name -> name -> DC name data
+    | negDc : DC name data -> DC name data.
 
     Notation "a @ b" := (andDc a b)(no associativity, at level 69).
     Notation "a $ b" := (orDc a b) (no associativity, at level 69).
 
-    Definition evalDC (po: option port) (d : option data) : bool :=
+    Definition evalDC (po: option tds) (d : data) : bool :=
        match po with
        | Some p => if (dataAssignment p(index p) == d) then true else false
        | None => false
        end.
+
     Lemma evalDCSound : forall po, forall d, evalDC po d = true <-> exists x, po = Some x /\ 
       dataAssignment x(index x) = d.
     Proof.
     split.
     - intros. destruct po. simpl in H2. destruct equiv_dec in H2.
-    + exists p. inversion e. auto.
+    + exists t. inversion e. auto.
     + inversion H2.
     + inversion H2.
     - intros. destruct H2. destruct H2. rewrite H2. unfold evalDC. rewrite H3. destruct equiv_dec.
       reflexivity. congruence.
     Defined.
 
-    (* The following definition searches for a port in a set of ports, returning it if it exists and None otherwise *)
-    Fixpoint retrievePortFromInput (s:set port) (n: name) :=
-      match s with
+
+    (* The following definition searches for a tds in a set of tds, returning it if it exists and None otherwise *)
+    Fixpoint retrievePortFromInput (tds:set tds) (n: name) :=
+      match tds with
       | [] => None
       | a::t => if (n == id a) then Some a else retrievePortFromInput t n
       end.
-    Lemma retrievePortFromInputSound : forall s:set port, forall n: name,forall a, retrievePortFromInput s n = Some a
-    -> In a s /\ n = id a.
+    Lemma retrievePortFromInputSound : forall tds:set tds, forall n: name,forall a, retrievePortFromInput tds n = Some a
+    -> In a tds /\ n = id a.
     Proof.
     - intros. 
-    + induction s. inversion H2.
+    + induction tds0. inversion H2.
     simpl in H2. destruct equiv_dec in H2. inversion e. split. inversion H2. simpl. auto. inversion H2. reflexivity.
-    apply IHs in H2. split. simpl. destruct H2. right. exact H2. destruct H2. exact H3. Defined.
+    apply IHtds0 in H2. split. simpl. destruct H2. right. exact H2. destruct H2. exact H3. Defined.
 
-    Definition eqDataPorts (n1: name) (n2: name) (s: set port) :=
-      match (retrievePortFromInput s n1) with
-      | Some a => match (retrievePortFromInput s n2) with
+    Definition eqDataPorts (n1: name) (n2: name) (theta: set tds) :=
+      match (retrievePortFromInput theta n1) with
+      | Some a => match (retrievePortFromInput theta n2) with
                   | Some b => if (dataAssignment a(index a)) == (dataAssignment b(index b)) then true else false
                   | None => false
                   end
       | None => false
       end.
 
-    Lemma eqDataPortsSound : forall n1, forall n2, forall s , eqDataPorts n1 n2 s = true <-> 
-      exists a, retrievePortFromInput s n1 = Some a /\ exists b, retrievePortFromInput s n2 = Some b 
+    Lemma eqDataPortsSound : forall n1, forall n2, forall tds , eqDataPorts n1 n2 tds = true <-> 
+      exists a, retrievePortFromInput tds n1 = Some a /\ exists b, retrievePortFromInput tds n2 = Some b 
       /\ (dataAssignment a(index a)) = (dataAssignment b(index b)).
     Proof.
     split.
-    - intros. unfold eqDataPorts in H2. case_eq (retrievePortFromInput s n1). 
-      case_eq (retrievePortFromInput s n2).
+    - intros. unfold eqDataPorts in H2. case_eq (retrievePortFromInput tds0 n1). 
+      case_eq (retrievePortFromInput tds0 n2).
     + intros. rewrite H3 in H2.  rewrite H4 in H2. destruct equiv_dec in H2. inversion e.
-      exists p0. split. reflexivity. exists p. split. reflexivity. assumption.
+      exists t0. split. reflexivity. exists t. split. reflexivity. assumption.
       inversion H2.
     + intros. rewrite H4 in H2. rewrite H3 in H2. inversion H2.
     + intros. rewrite H3 in H2. inversion H2.
@@ -151,24 +183,24 @@ Module ConstraintAutomata.
       unfold eqDataPorts. rewrite H2. rewrite H3. rewrite H4. destruct equiv_dec. reflexivity. congruence.
   Defined.
 
-    Definition transformDC (transform: option data -> option data) (n1: name) (n2: name) (s:set port) :=
-      match (retrievePortFromInput s n1) with
-      | Some a => match (retrievePortFromInput s n2) with
+    Definition transformDC (transform: data -> data) (n1: name) (n2: name) (tds:set tds) :=
+      match (retrievePortFromInput tds n1) with
+      | Some a => match (retrievePortFromInput tds n2) with
                   | Some b => if transform((dataAssignment a(index a))) == (dataAssignment b(index b)) then true else false
                   | None => false
                   end
       | None => false
       end.
 
-    Lemma transformDCsound : forall transform, forall n1, forall n2, forall s, transformDC transform n1 n2 s = true <->
-      exists a, retrievePortFromInput s n1 = Some a /\ exists b, retrievePortFromInput s n2 = Some b 
+    Lemma transformDCsound : forall transform, forall n1, forall n2, forall tds, transformDC transform n1 n2 tds = true <->
+      exists a, retrievePortFromInput tds n1 = Some a /\ exists b, retrievePortFromInput tds n2 = Some b 
       /\ transform((dataAssignment a(index a))) = (dataAssignment b(index b)).
     Proof.
     split.
-    - intros. unfold transformDC in H2. case_eq (retrievePortFromInput s n1). 
-      case_eq (retrievePortFromInput s n2).
+    - intros. unfold transformDC in H2. case_eq (retrievePortFromInput tds0 n1). 
+      case_eq (retrievePortFromInput tds0 n2).
     + intros. rewrite H3 in H2.  rewrite H4 in H2. destruct equiv_dec in H2. inversion e.
-      exists p0. split. reflexivity. exists p. split. reflexivity. assumption.
+      exists t0. split. reflexivity. exists t. split. reflexivity. assumption.
       inversion H2.
     + intros. rewrite H4 in H2. rewrite H3 in H2. inversion H2.
     + intros. rewrite H3 in H2. inversion H2.
@@ -176,34 +208,34 @@ Module ConstraintAutomata.
       unfold transformDC. rewrite H2. rewrite H3. rewrite H4. destruct equiv_dec. reflexivity. congruence.
     Defined.
 
-    Fixpoint evalCompositeDc (s:set port) (dc: DC) : bool :=
+    Fixpoint evalCompositeDc (tds:set tds) (dc: DC name data) : bool :=
       match dc with
-      | tDc => true
-      | dc a b => evalDC (retrievePortFromInput s a) (b)
-      | eqDc a b => eqDataPorts a b s
-      | andDc a b => evalCompositeDc s a && evalCompositeDc s b
-      | orDc a b => evalCompositeDc s a || evalCompositeDc s b
-      | trDc transform a b  => transformDC transform a b s
-      | negDc a => negb (evalCompositeDc s a)
+      | tDc _ _ => true
+      | dc a b => evalDC (retrievePortFromInput tds a) (b)
+      | eqDc _ a b => eqDataPorts a b tds
+      | andDc a b => evalCompositeDc tds a && evalCompositeDc tds b
+      | orDc a b => evalCompositeDc tds a || evalCompositeDc tds b
+      | trDc transform a b  => transformDC transform a b tds
+      | negDc a => negb (evalCompositeDc tds a)
       end.  
 
-      Lemma evalCompositeDcSound : forall s, forall dca: DC, evalCompositeDc s dca = true <-> 
-      dca = tDc \/ 
-      (exists a, exists b, dca = dc a b /\ (evalDC (retrievePortFromInput s a) b) = true ) \/
-      (exists a, exists b, dca = eqDc a b /\ eqDataPorts a b s = true) \/
-      (exists a, exists b, dca = andDc a b /\ evalCompositeDc s a && evalCompositeDc s b = true) \/
-      (exists a,exists b, dca = orDc a b /\ evalCompositeDc s a || evalCompositeDc s b = true) \/
-      (exists a, exists b, exists tr, dca = trDc tr a b /\ transformDC tr a b s = true) \/
-      (exists a, dca = negDc a /\ negb (evalCompositeDc s a) = true).
+      Lemma evalCompositeDcSound : forall tds, forall dca: DC name data, evalCompositeDc tds dca = true <-> 
+      dca = tDc _ _ \/ 
+      (exists a, exists b, dca = dc a b /\ (evalDC (retrievePortFromInput tds a) b) = true ) \/
+      (exists a, exists b, dca = eqDc _ a b /\ eqDataPorts a b tds = true) \/
+      (exists a, exists b, dca = andDc a b /\ evalCompositeDc tds a && evalCompositeDc tds b = true) \/
+      (exists a,exists b, dca = orDc a b /\ evalCompositeDc tds a || evalCompositeDc tds b = true) \/
+      (exists a, exists b, exists tr, dca = trDc tr a b /\ transformDC tr a b tds = true) \/
+      (exists a, dca = negDc a /\ negb (evalCompositeDc tds a) = true).
       Proof.  
       split.
       - intros. destruct dca.
       + left. reflexivity.
-      + simpl in H2. right. left. exists n. exists o. auto.
+      + simpl in H2. right. left. exists n. exists d. auto.
       + simpl in H2. right. right. left. exists n. exists n0. auto.
       + simpl in H2. right. right. right. left.  exists dca1. exists dca2. auto.
       + simpl in H2. right. right. right. right. left. exists dca1. exists dca2. auto.
-      + simpl in H2. right. right. right. right. right. left. exists n. exists n0. exists o. auto.
+      + simpl in H2. right. right. right. right. right. left. exists n. exists n0. exists d. auto.
       + simpl in H2. repeat right. exists dca.  auto.
       - intros. destruct H2.
       + rewrite H2. reflexivity.
@@ -218,14 +250,14 @@ Module ConstraintAutomata.
     Record constraintAutomata : Type := CA {
       Q : set state;
       N : set name;
-      T : state -> set (set (name) * DC * set(state));
+      T : state -> set (set (name) * DC name data * state);
       Q0 : set state;
     }.
 
     Fixpoint returnSmallerNumber (m:QArith_base.Q) (l:set QArith_base.Q) :=
       match l with
       | [] => m
-      | a::t => if ((a <? m) == true) then 
+      | a::t => if ((a <? m)) then 
                    returnSmallerNumber a t else returnSmallerNumber m t
       end.
     Open Scope Q_scope.
@@ -238,621 +270,812 @@ Module ConstraintAutomata.
     unfold returnSmallerNumber in H2. congruence.
     simpl in H2. split.
     discriminate.
-    destruct equiv_dec in H2. inversion e. exists a. simpl; auto. 
-    apply IHl in H2. destruct H2. destruct H3. destruct H3. exists x. split. simpl. right. exact H3.
-    exact H4.
+    case_eq (a <? m). intros. rewrite H3 in H2. exists a. simpl. auto.
+    intros. rewrite H3 in H2. apply IHl in H2. destruct H2. repeat (destruct H4).
+    exists x. split. simpl. right. exact H4. exact H5.
     Defined.
-
-    Definition hasData (p:port) (k:nat) :=
-      match (dataAssignment p(k)) with
-      | Some a => true
-      | None => false
-      end.
-
-    Lemma hasDataSound : forall p, forall k, hasData p k = true <-> exists data, dataAssignment p(k) = Some data.
-    Proof.
-    intros. split.
-    - intros Ha. unfold hasData in Ha. destruct dataAssignment. exists d. reflexivity.
-      inversion Ha.
-    - intros Ha. unfold hasData. inversion Ha. rewrite H2. reflexivity.
-    Defined.
-
 
     Notation "x |> f" := (f x) (at level 69, only parsing).
 
     Close Scope Q_scope.
 
-    Definition getThetaTimeCandidate (p:port) :=
+    Definition getThetaTimeCandidate (p:tds) :=
       [timeStamp p(index(p))].
 
-    Fixpoint getAllThetaTimes (s: set port) :=
-      match s with
+    Fixpoint getAllThetaTimes (theta: set tds) :=
+      match theta with
       | [] => []
       | a::t => getThetaTimeCandidate a++getAllThetaTimes t
       end.
-    Lemma getAllThetaTimesSound : forall s: set port, getAllThetaTimes s <> [] <-> exists a, In a s.
+    Lemma getAllThetaTimesSound : forall s: set tds, getAllThetaTimes s <> [] <-> exists a, In a s.
     Proof.
     split.
-    - intros. destruct s. simpl in H2. congruence. exists p. simpl. auto.
+    - intros. destruct s. simpl in H2. congruence. exists t. simpl. auto.
     - intros. destruct s. inversion H2. inversion H3. simpl. discriminate.
     Defined.
 
-  Check getAllThetaTimes.
-
-    Definition getNextThetaTime (l: set QArith_base.Q) :=
+    Definition minimum (l: set QArith_base.Q) :=
        returnSmallerNumber (hd (Qmake 0 1) l) (tl l).
 
-    Program Fixpoint count_into_list (n:nat) :=
-      match n with
-      | 0 => 0::nil
-      | S n => count_into_list n ++ [S n]
-      end.
+    Definition nextTime (theta:set tds) :=
+      minimum(getAllThetaTimes theta).
 
-    Definition thetaTime (s:set port) (k:nat) :=
-      getNextThetaTime(getAllThetaTimes s).
+    Definition timeStampEqThetaTime (theta:set tds) (a:tds) :=
+      (timeStamp a(index a) =? nextTime (theta)).
 
-    Definition timeStampEqThetaTime (s:set port) (k:nat) (a:port) :=
-      if ((timeStamp a(index a) =? thetaTime (s) (k)) == true) then true else false.
-
-    Lemma timeStampEqThetaTimeSound : forall s, forall k, forall a, timeStampEqThetaTime s k a = true <-> 
-      ((timeStamp a(index a) =? thetaTime (s) (k)) = true).
+    Lemma timeStampEqThetaTimeSound : forall s, forall a, timeStampEqThetaTime s a = true <-> 
+      ((timeStamp a(index a) =? nextTime (s)) = true).
     Proof.
     split.
-    - intros. unfold timeStampEqThetaTime in H2. destruct equiv_dec in H2.
-      inversion e. reflexivity.
-      inversion H2.
+    - intros. unfold timeStampEqThetaTime in H2. exact H2.
     - intros. unfold timeStampEqThetaTime. rewrite H2. reflexivity.
     Defined.
 
-    Fixpoint thetaN (ca: set port) (k:nat) (s:set port) : set name := 
-      match s with
-      | a::t => if (hasData a k == true) then
-                  if (timeStampEqThetaTime ca k a == true) then
-                     id a :: thetaN ca k t
-                   else thetaN ca k t
-                else thetaN ca k t
+    Fixpoint nextNames (theta: set tds) (theta2:set tds) : set name := 
+      match theta2 with
+      | a::t => if (timeStampEqThetaTime theta a ) then
+                    id a :: nextNames theta t
+                else nextNames theta t
       | []   => []
       end.
 
-    Lemma thetaNSound : forall ca, forall k, forall s, thetaN ca k s <> [] <-> 
-    (exists a, In a s /\ hasData a(k) = true /\ timeStampEqThetaTime ca k a = true).
+    Lemma nextNamesSound : forall theta, forall theta2, nextNames theta theta2 <> [] <-> 
+    (exists a, In a theta2 /\ timeStampEqThetaTime theta a = true).
     Proof.
     split.
-    - intros. induction s.
+    - intros. induction theta2.
     + simpl in H2. congruence.
-    + simpl in H2. destruct equiv_dec in H2. destruct equiv_dec in H2.
-      exists a. split. simpl;auto. split. inversion e. reflexivity. inversion e0. reflexivity.
-      apply IHs in H2. destruct H2. destruct H2. destruct H3. exists x. split. simpl;auto.
-      split. exact H3. exact H4.
-      apply IHs in H2. destruct H2.  destruct H2. destruct H3. exists x. split. simpl;auto.
-      split. exact H3. exact H4. 
-    -  intros. induction s. 
+    + simpl in H2. case_eq (timeStampEqThetaTime theta a).
+    { intros. exists a. split. simpl;auto. exact H3. }
+    { intros. rewrite H3 in H2. apply IHtheta2 in H2. destruct H2. destruct H2.
+      exists x. split. simpl;auto. exact H4. }
+    -  intros. induction theta2. 
     + destruct H2.  destruct H2. inversion H2.
-    + simpl. destruct equiv_dec. destruct equiv_dec. discriminate.
-      apply IHs. destruct H2. destruct H2. simpl in H2. destruct H2. destruct H3. rewrite <- H2 in H4. 
-      congruence. exists x. split. exact H2. exact H3.
-      apply IHs. destruct H2. destruct H2. simpl in H2. destruct H2. destruct H3. rewrite <- H2 in H4. 
-      congruence. exists x. split. exact H2. exact H3. Defined.
+    + simpl. case_eq (timeStampEqThetaTime theta a). intros. discriminate.
+      intros. apply IHtheta2. destruct H2. destruct H2. simpl in H2. destruct H2.  rewrite <- H2 in H4. 
+      congruence. exists x. split. exact H2. exact H4.
+    Defined. 
+    
+    Definition thetaN (theta: set tds) :=
+      nextNames (theta) (theta).
 
-    Fixpoint portsWithData (ca: set port) (k:nat) (s:set port) : set((name * option data)) := 
-      match s with
-      | a::t => if (hasData a k == true) then
-                  if (timeStampEqThetaTime ca k a == true) then
-                     ((id a) , (dataAssignment a(index(a)))) :: portsWithData ca k t
-                   else portsWithData ca k t
-                else portsWithData ca k t
+    Fixpoint nextData (theta: set tds) (theta2:set tds) : set((name * data)) := 
+      match theta2 with
+      | a::t => if (timeStampEqThetaTime theta a) then
+                   ((id a) , (dataAssignment a(index(a)))) :: nextData theta t
+                else nextData theta t
       | []   => []
       end.
 
-    Lemma portsWithDataSound : forall ca, forall k, forall s, portsWithData ca k s <> [] <-> 
-    (exists a, In a s /\ hasData a(k) = true /\ timeStampEqThetaTime ca k a = true).
+    Lemma nextDataSound : forall theta, forall theta2, nextData theta theta2 <> [] <-> 
+    (exists a, In a theta2 /\ timeStampEqThetaTime theta a = true).
     Proof.
     split.
-    - intros. induction s.
+    - intros. induction theta2.
     + simpl in H2. congruence.
-    + simpl in H2. destruct equiv_dec in H2. destruct equiv_dec in H2.
-      exists a. split. simpl;auto. split. inversion e. reflexivity. inversion e0. reflexivity.
-      apply IHs in H2. destruct H2. destruct H2. destruct H3. exists x. split. simpl;auto.
-      split. exact H3. exact H4.
-      apply IHs in H2. destruct H2.  destruct H2. destruct H3. exists x. split. simpl;auto.
-      split. exact H3. exact H4. 
-    -  intros. induction s. 
+    + simpl in H2. case_eq (timeStampEqThetaTime theta a).
+    { intros. exists a. split. simpl;auto. exact H3. }
+    { intros. rewrite H3 in H2. apply IHtheta2 in H2. destruct H2. destruct H2.
+      exists x. split. simpl;auto. exact H4. }
+    -  intros. induction theta2. 
     + destruct H2.  destruct H2. inversion H2.
-    + simpl. destruct equiv_dec. destruct equiv_dec. discriminate.
-      apply IHs. destruct H2. destruct H2. simpl in H2. destruct H2. destruct H3. rewrite <- H2 in H4. 
-      congruence. exists x. split. exact H2. exact H3.
-      apply IHs. destruct H2. destruct H2. simpl in H2. destruct H2. destruct H3. rewrite <- H2 in H4. 
-      congruence. exists x. split. exact H2. exact H3. Defined.
-
-    Definition thetaDelta (k : nat) (po: set port) := 
-      portsWithData po k po.
-    Check thetaDelta.
+    + simpl. case_eq (timeStampEqThetaTime theta a). intros. discriminate.
+      intros. apply IHtheta2. destruct H2. destruct H2. simpl in H2. destruct H2.  rewrite <- H2 in H4. 
+      congruence. exists x. split. exact H2. exact H4.
+    Defined. 
 
     Close Scope Q_scope.
 
-    Definition derivative (p: port) := mkport (id p) (dataAssignment p) (timeStamp p)
-        (portCond p) (S (index p)).
+    Definition derivative (p: tds) := mktds (id p) (dataAssignment p) (timeStamp p)
+        (tdsCond p) (S (index p)).
 
-    Lemma derivative_sound : forall p, derivative p = mkport (id p) (dataAssignment p) (timeStamp p)
-        (portCond p) ( S(index p)).
+    Lemma derivative_sound : forall p, derivative p = mktds (id p) (dataAssignment p) (timeStamp p)
+        (tdsCond p) ( S(index p)).
     Proof.
     reflexivity.
     Defined.
 
-    Fixpoint derivativePortInvolved (s:set name) (a: port)  :=
+    Fixpoint derivativePortInvolved (s:set name) (a: tds)  :=
       match s with
       | [] => [a] 
       | x::t => if x == id a then [derivative(a)]
                 else derivativePortInvolved t a
       end.
 
-    Definition allDerivativesFromPortsInvolved (names: set name) (ports:set port) : set port :=
-      flat_map (derivativePortInvolved names) ports.
+    Definition allDerivativesFromPortsInvolved (names: set name) (theta:set tds) : set tds :=
+      flat_map (derivativePortInvolved names) theta.
 
-    Definition portsDerivative (names: set name) (input: set port) := 
-      allDerivativesFromPortsInvolved names input. 
+    Definition portsDerivative (names: set name) (theta: set tds) := 
+      allDerivativesFromPortsInvolved names theta. 
 
-    Fixpoint portsOutsideTransition (input: port) (ports : set name) :=
-      match ports with
+    Fixpoint portsOutsideTransition (p: tds) (portNames : set name) :=
+      match portNames with
        | [] => true
-       | a::t => if (id input <> a) then portsOutsideTransition input t else false
+       | a::t => if (id p <> a) then portsOutsideTransition p t else false
       end.
 
-    Lemma portsOutsideTransitionSound : forall input, forall ports, portsOutsideTransition input ports = false <->
-      (exists b, In b ports /\ (id input = b)).
+    Lemma portsOutsideTransitionSound : forall p, forall portNames, portsOutsideTransition p portNames = false <->
+      (exists b, In b portNames /\ (id p = b)).
     Proof.
     split.
-    - intros. induction ports.
+    - intros. induction portNames.
     + simpl in H2. inversion H2.
-    + simpl in H2. destruct nequiv_dec in H2. apply IHports in H2.
+    + simpl in H2. destruct nequiv_dec in H2. apply IHportNames in H2.
       repeat destruct H2. exists x. split.
       simpl;auto.
       exact H3.
       inversion e. exists a.
       split. simpl;auto.
       exact H3.
-    - intros. induction ports.
+    - intros. induction portNames.
     + repeat destruct H2.
-    + simpl. destruct nequiv_dec. apply IHports. repeat destruct H2. congruence. exists x. split; assumption.
+    + simpl. destruct nequiv_dec. apply IHportNames. repeat destruct H2. congruence. exists x. split; assumption.
       reflexivity. 
     Defined.
+  
+    Fixpoint step' (theta : set tds) (portNames: set name)
+     (transitions: set(set name * DC name data * state)) : set state :=
+     match transitions with
+     | [] => []
+     | a::t => if (set_eq (portNames)((fst(fst(a))))) 
+                   && (evalCompositeDc (theta) (snd(fst(a)))) then snd(a)::step' theta portNames t
+                   else step' theta portNames t
+     end.
 
-
-    Fixpoint retrievePortsOutsideTransition (input: set port) (ports : set name) :=
-      match input with
-      | [] => []
-      | a::x => if (portsOutsideTransition a ports) == true then a::retrievePortsOutsideTransition x ports
-                else retrievePortsOutsideTransition x ports
-      end.
-    Check retrievePortsOutsideTransition.
-
-    Lemma retrievePortsOutsideTransitionSound : forall input, forall ports,
-    retrievePortsOutsideTransition input ports <> [] <-> exists a, portsOutsideTransition a ports = true /\
-    In a input.
-    Proof.
-    split.
-    - intros. induction input.
-    + simpl in H2. congruence.
-    + simpl in H2. destruct equiv_dec in H2. inversion e.
-      exists a. split. reflexivity.  simpl;auto.
-      apply IHinput in H2. destruct H2. exists x. destruct H2.
-      split. assumption.
-      simpl;auto.
-    - intros. induction input. destruct H2. destruct H2. 
-    + inversion H3. 
-    + simpl. destruct equiv_dec.
-      discriminate. 
-      apply IHinput. destruct H2.
-      destruct H2. simpl in H3.
-      destruct H3. rewrite <- H3 in H2. congruence.
-      exists x. split. exact H2. exact H3. Defined.
-
-
-    Fixpoint hasDataInThetaDelta (p: port) (thetadelta: set (name * option data)) :=
-      match thetadelta with
-      | [] => false
-      | a::t => if ((id p ==(fst(a)))) then
-                    if snd(a) <> None then true 
-                    else hasDataInThetaDelta (p) (t)
-                else hasDataInThetaDelta p t
-      end.
-
-    Lemma hasDataInThetaDeltaSound : forall p, forall thetadelta, hasDataInThetaDelta p thetadelta = true <-> 
-      exists a, In a thetadelta /\ (id p = (fst(a))) /\ (snd(a)<> None).
-    Proof.
-    split.
-    - intros. induction thetadelta.
-    + inversion H2.
-    + simpl in H2. destruct equiv_dec in H2. destruct nequiv_dec in H2. inversion e.
-      exists a. split.
-      simpl;auto.
-      split. exact H4.
-      congruence.
-      apply IHthetadelta in H2. destruct H2. destruct H2. exists x. split.
-      simpl;auto. exact H3.
-      apply IHthetadelta in H2. destruct H2. destruct H2. exists x. split.
-      simpl;auto. exact H3.
-    - intros. induction thetadelta.
-    + repeat destruct H2. 
-    +  destruct H2. destruct H2. destruct H3. simpl in H2. 
-       simpl. destruct equiv_dec. destruct nequiv_dec. reflexivity. inversion e0. 
-       destruct H2. rewrite H2 in H6. congruence.
-       apply IHthetadelta. exists x. inversion e.
-       repeat split; assumption. apply IHthetadelta.
-       destruct H2. rewrite <- H2 in H3. congruence.
-       exists x. repeat split;assumption.
+    Lemma step'_sound : forall theta, forall portNames, forall transitions, step' theta portNames transitions <> [] -> exists a,
+    In a transitions /\ (set_eq (portNames)((fst(fst(a)))))
+                   && (evalCompositeDc (theta) (snd(fst(a)))) = true.
+    Proof. 
+    - intros. induction transitions. simpl in H2. congruence. simpl in H2. 
+    case_eq (set_eq (portNames)((fst(fst(a))))). 
+    case_eq (evalCompositeDc theta (snd (fst a))). intros.
+    + exists a. split. simpl;auto. rewrite H3. rewrite H4. reflexivity.
+    + intros. rewrite H3 in H2. rewrite H4 in H2. apply IHtransitions in H2.
+      destruct H2. destruct H2. exists x. split. simpl;auto. exact H5.
+    + intros. rewrite H3 in H2. apply IHtransitions in H2.
+      destruct H2. destruct H2. exists x. split. simpl;auto. exact H4.
     Defined.
 
-    Fixpoint checkPorts (t:set port) (thetadelta: set (name * option data)) :=
-      match t with
-      | [] => true
-      | a::x => if (negb (hasDataInThetaDelta a thetadelta) == true) then checkPorts x thetadelta
-                else false
-      end.
-
-    Lemma checkPortsSound : forall t, forall thetadelta, checkPorts t thetadelta = false <->
-      exists a, In a t /\ negb (hasDataInThetaDelta a thetadelta) = false.
-    Proof.
-    split.
-    - intros. induction t.
-    + inversion H2.
-    + simpl in H2. destruct equiv_dec in H2. apply IHt in H2. repeat destruct H2.
-      exists x. split. simpl;auto. exact H3.
-      exists a. destruct hasDataInThetaDelta. split. simpl;auto. reflexivity. simpl in c. congruence.
-    - intros. induction t.
-    + repeat destruct H2.
-    +  simpl. destruct equiv_dec. apply IHt. destruct H2. destruct H2. simpl in H2. destruct H2.
-      inversion e. rewrite H2 in H5. congruence.
-      exists x. split. exact H2. exact H3. reflexivity.
-      Defined.
-
-    Definition onlyPortsInvolvedContainsData (ports : set name) 
-      (k : nat) (input : set port) :=
-      checkPorts (retrievePortsOutsideTransition (input) ports) (thetaDelta (k) (input)).
-
-    Definition retrievePortsFromThetaN (k : nat) (input: set port) :=
-      thetaN (input) (k) (input).
-
-   Check retrievePortsFromThetaN.
-
-    Fixpoint step' (k : nat) (input : set port) (ports: set name)
-     (s: set(set name * DC * set(state))) :=
-     match s with
-     | [] => []
-     | a::t => if (set_eq (ports)((fst(fst(a))))) && 
-                  (onlyPortsInvolvedContainsData (fst(fst(a))) k input)
-                   && (evalCompositeDc (input) (snd(fst(a)))) == true then snd(a)++step' k input ports t
-                   else step' k input ports t
-     end.
-    Check step'.
-
-    Lemma step'_sound : forall k, forall input, forall ports, forall s, step' k input ports s <> [] -> exists a,
-    In a s /\ (set_eq (ports)((fst(fst(a))))) && (onlyPortsInvolvedContainsData (fst(fst(a))) k input)
-                   && (evalCompositeDc (input) (snd(fst(a)))) = true.
-    Proof. 
-    - intros. induction s. simpl in H2. congruence. simpl in H2. destruct equiv_dec in H2. inversion e.
-    + exists a. split. simpl;auto. reflexivity.
-    + apply IHs in H2. destruct H2. destruct H2. exists x. split. simpl;auto. exact H3. Defined.
-
-    Definition stepAux (ca:constraintAutomata) (k : nat) (input:set port) (ports:set name) (s: state) :=
-      step' k input ports (T ca s).
+    Definition stepAux (ca:constraintAutomata) (theta:set tds) (portNames:set name) (s: state) 
+    : set state :=
+      step' theta portNames (T ca s).
 
     (* We apply the step to every state in the given configuration:                     *)
-    Definition stepa (ca:constraintAutomata) (s: set state) (k : nat) (input:set port) (ports: set name):=
-     (ports, flat_map (stepAux ca k input ports) s).
+    Definition stepa (ca:constraintAutomata) (s: set state) (theta:set tds) (portNames: set name) 
+    : set name * set state :=
+     (portNames, flat_map (stepAux ca theta portNames) s).
 
-    Check stepa.
-
-    Definition step (ca:constraintAutomata) (s: set state) (k : nat) (input:set port) :=
-      stepa ca s k input (retrievePortsFromThetaN k input).
-
+    Definition step (ca:constraintAutomata) (s: set state) (theta:set tds) : set name * set state :=
+      stepa ca s theta (thetaN theta).
 
     Definition run' (ca:constraintAutomata)  : 
-      set port -> list nat -> set state -> set (set state) -> set (set state) :=
-      fix rec input k acc resp :=
+      set tds -> nat -> set state -> set (set state) -> set (set state) :=
+      fix rec theta k initialStates trace := 
         match k with 
-          | [] => resp
-          | a::t => resp ++ [snd (step ca acc a input)]
+          | 0 => trace
+          | S m => trace ++ [snd (step ca initialStates theta)]
                     |> rec
-                      (flat_map(derivativePortInvolved(fst((step ca acc a input)))) input) t (snd (step ca acc a input))
+                      (flat_map(derivativePortInvolved(fst((step ca initialStates theta)))) theta) m (snd (step ca initialStates theta))
         end.
 
-    Definition run (ca:constraintAutomata) (input: set port) (k : nat) :=
-      run' ca input (count_into_list k) (Q0 ca) [Q0 ca].
+    Definition run (ca:constraintAutomata) (theta: set tds) (k : nat) :=
+      run' ca theta k (Q0 ca) [Q0 ca].
+
+  (* We define a function that returns the input theta post processed by the automaton. Intuitively, *)
+  (* it is similar to run but instead of accumulating states, it returns theta's k-th derivative     *)
+
+    Definition tdsDerivate (ca:constraintAutomata)  : 
+      set tds -> nat -> set state -> set tds :=
+      fix rec theta k initialStates := 
+        match k with 
+          | 0 => theta
+          | S m => rec (flat_map (derivativePortInvolved(fst((step ca initialStates theta)))) theta) m (snd(step ca initialStates theta)) 
+        end.
+
+  (* And a version of a run which returns only the last state reached *)
+    Definition lastReachedStates (ca:constraintAutomata) (theta: set tds) (k : nat) : set state :=
+      last (run ca theta k) (ConstraintAutomata.Q0 ca).
+
+  (* We define some functions to retrieve data from transitions, in order to prove *)
+  (* properties about behavior of automata                                         *)
+
+    Fixpoint retrievePortsFromRespTransitions (s : set (set (name) * DC name data * state)) :=
+    match s with
+    | [] => []
+    | a::t => set_union equiv_dec (fst (fst a) ) (retrievePortsFromRespTransitions t)
+    end.
+
+    Definition portsOfTransition (ca: constraintAutomata) (s : state) :=
+      retrievePortsFromRespTransitions (ConstraintAutomata.T ca s).
+
+  (* We define acceptance for infinite runs as Baier et al. propose
+  Terminar melhor essa definição: talvez realmente meter a noção de aceitação de baier et al.*)
+
+  Definition accepting (ca: constraintAutomata) (theta: set tds) : Prop :=
+    forall k, forall final, In (final) (lastReachedStates ca theta k) -> (*/\ *)
+                        exists t, In t (step' (tdsDerivate ca theta k (ConstraintAutomata.Q0 ca)) (*(theta : set tds) *)
+                        (thetaN (tdsDerivate ca theta k (ConstraintAutomata.Q0 ca)))(*portNames: set name*)
+                        ((ConstraintAutomata.T ca final))) . (*transitions : set(set name * DC name data * state))*) 
 
 
+
+  (* Bisimulation as boolean verification *)
+
+
+  (* We filter the transition to be compared with a transition that contains the same name set *)
+  Fixpoint getTransition (portNames: set name) (t2 : set (set(name) * DC name data * state)) :=
+    match t2 with
+    | [] => [] 
+    | a::t => if (set_eq portNames (fst(fst(a)))) then a::getTransition portNames t else getTransition portNames t
+    end. 
+
+  (* We need to evalate whether the next reached states are also equivalent. Then, we need to store *)
+  (* pairs of states to be evaluated *)
+  Fixpoint getReachedStatesFromPair (t1 : (set(name) * DC name data * state)) (setT2 : set (set(name) * DC name data * state)) :=
+    match setT2 with
+    | [] => []
+    | a::nextT2 =>  set_add equiv_dec (snd(t1),snd(a)) (getReachedStatesFromPair t1 nextT2)
+    end.
+
+  (* Check whether exists a transition with port names equal to the port name of a single transition of A1 *)
+  Fixpoint iterateTransitionsQ1A1 (ca1: constraintAutomata) (ca2: constraintAutomata) (q1: state) (q2: state) 
+    (setT1 : set (set(name) * DC name data * state)) (setT2: set (set(name) * DC name data * state)) 
+    (acc: set (state * state)) :=
+    match setT1 with
+    | [] => (q1,q2)::acc 
+    | a::t => if set_eq ((getReachedStatesFromPair (a) (getTransition (fst(fst(a))) (setT2)))) ([]) then [] else 
+              ((getReachedStatesFromPair (a) (getTransition (fst(fst(a))) (setT2))))++ iterateTransitionsQ1A1 ca1 ca2 q1 q2 t setT2 acc
+    end.
+ 
+  (* Expanding the reached states *)
+  Definition iterateOverNextStates (ca1: constraintAutomata) (ca2: constraintAutomata) (acc : set (state * state))
+  (states : set (state * state)) :=
+    match states with
+    | [] => []
+    | a::t => iterateTransitionsQ1A1 ca1 ca2 (fst(a)) (snd(a)) (ConstraintAutomata.T ca1 (fst(a))) 
+              (ConstraintAutomata.T ca2 (snd(a))) acc 
+    end.
+
+  Fixpoint bisimilarStatesCa1ToCa2 (ca1: constraintAutomata) (ca2: constraintAutomata) (q1: state) (q2: state) 
+    (setT1 : set (set(name) * DC name data * state)) (setT2: set (set(name) * DC name data * state)) 
+    (acc: set (state * state)) :=
+    match setT1 with
+    | [] => (q1,q2)::acc
+    | a::t => if set_eq ((getReachedStatesFromPair (a) (getTransition (fst(fst(a))) (setT2)))) ([]) then [] else
+              bisimilarStatesCa1ToCa2 ca1 ca2 q1 q2 t setT2 acc
+    end.
+
+  (* Retrieving only the bisimilar states after each round. *)
+  Fixpoint retrieveCleanStates (ca1: constraintAutomata) (ca2: constraintAutomata)
+  (acc: set (state * state)) (states: set (state * state)) :=
+    match states with
+    | [] => []
+    | a::t => set_union equiv_dec (bisimilarStatesCa1ToCa2 ca1 ca2 (fst(a)) (snd(a)) (ConstraintAutomata.T ca1 (fst(a))) (ConstraintAutomata.T ca2 (snd(a))) acc)
+              (retrieveCleanStates ca1 ca2 acc t)
+    end. 
+  
+  (* Auxiliary definition that iterates over the set of (possible) bisimilar states, recursively verifying whether they indeed are bisimilar *)
+  Definition evaluateObtainedStates (ca1: constraintAutomata) (ca2: constraintAutomata) : nat -> set (state * state) -> 
+  set (state * state) -> set (state * state) :=
+    fix rec steps acc nextPairStates :=
+    match steps with
+    | 0 =>  acc
+    | S n =>
+            set_union equiv_dec (rec n acc (iterateOverNextStates ca1 ca2 acc nextPairStates)) 
+            (retrieveCleanStates ca1 ca2 acc ((iterateOverNextStates ca1 ca2 acc nextPairStates)))
+    end.
+
+  Fixpoint iterateOverA2States (ca1: constraintAutomata) (ca2: constraintAutomata) (q1: state) (q2: set (state)) 
+    (acc: set (state * state)) :=
+    match q2 with
+    | [] => acc
+    | a::t => evaluateObtainedStates ca1 ca2 (length(ConstraintAutomata.Q(ca1))) acc [(q1,a)]  
+              ++ iterateOverA2States ca1 ca2 q1 t acc
+    end.  
+
+  Fixpoint iterateOverA1States (ca1: constraintAutomata) (ca2: constraintAutomata) (q1: set (state)) (q2: set (state)) 
+  (acc: set (state * state)) : set (state * state) :=
+    match q1 with
+    | [] => acc
+    | a::t => iterateOverA2States ca1 ca2 a q2 acc ++ iterateOverA1States ca1 ca2 t q2 acc
+    end.
+
+  Fixpoint containsSymmetric (setPairs : set (state * state)) (setPairsFull: set (state * state)):=
+    match setPairs with
+    | [] => []
+    | a::t => match a with
+              | (q1,q2) => if existsb (fun x : (state * state) => match x with
+                                       |(a,b) => (equiv_decb a q2) && (equiv_decb b q1)  end) (setPairsFull) then (q1,q2)::containsSymmetric t setPairsFull
+                           else containsSymmetric t setPairsFull
+              end
+    end.
+
+  Definition bisimulationAux (ca1: constraintAutomata) (ca2: constraintAutomata) :=
+    (iterateOverA1States ca1 ca2 (ConstraintAutomata.Q0 ca1) (ConstraintAutomata.Q0 ca2) []) ++ 
+    (iterateOverA1States ca2 ca1 (ConstraintAutomata.Q0 ca2) (ConstraintAutomata.Q0 ca1) []).
+
+  (* bisimulation is commutative *)
+  Lemma bisimulationAuxCommutative : forall ca1, forall ca2, forall a, 
+   (In a (bisimulationAux ca1 ca2)) <-> (In a (bisimulationAux ca2 ca1)).
+  Proof.
+  intros.
+  split.
+  - intros. unfold bisimulationAux. unfold bisimulationAux in H2. apply in_or_app.
+    apply in_app_or in H2. destruct H2. right. exact H2. left. exact H2.
+  - intros. unfold bisimulationAux. unfold bisimulationAux in H2. apply in_or_app.
+    apply in_app_or in H2. destruct H2. right. exact H2. left. exact H2.
+  Defined.
+
+  (* We compute if the relation is symmetric *)
+  Fixpoint isSymmetricAux (setPairs : set (state * state)) (setPairsFull: set (state * state)) :=
+    set_eq (setPairs) (containsSymmetric (setPairs) setPairsFull).
+
+  Definition isSymmetric (setPairs : set (state * state)) :=
+    if isSymmetricAux (setPairs) (setPairs) then setPairs else [].
+
+
+  (* We retrieve possible pair of states that can be transitive within R *)
+ (* Fixpoint retrieveCandidatesTransitivity (setPairs : set (state * state)) (setPairsFull: set (state * state)) :=
+    match setPairs with
+    | [] => []
+    | pairStates::t => match pairStates with
+                       | (a, b) => set_union equiv_dec (flat_map (fun x : (state * state) => match x with 
+                                    |(a',b') => if (equiv_decb b a') then [(a,b')]
+                                                else [] end) setPairsFull) (retrieveCandidatesTransitivity t setPairsFull)
+              end
+    end.
+
+  Check retrieveCandidatesTransitivity.
+
+  (* We check the transitivity of the obtained relation by computing pairs to which the transitivity holds.*)
+  Fixpoint computeTransitivity (ca1: constraintAutomata) (ca2: constraintAutomata) 
+  (setPairs : set (state * state)) (setPairsFull: set (state * state)) :=
+  match setPairs with
+  | [] => setPairsFull
+  | pairStates::t => match pairStates with
+                     | (a,b) => if (match ConstraintAutomata.T ca2 b with
+                                    | [] => true
+                                    | _ => false
+                                    end) 
+                                then set_union equiv_dec (bisimilarStatesCa1ToCa2 ca1 ca2 a b 
+                                  (ConstraintAutomata.T ca2 b) (ConstraintAutomata.T ca1 a) [])
+                                     (computeTransitivity ca1 ca2 t setPairsFull)
+                                else set_union equiv_dec (bisimilarStatesCa1ToCa2 ca1 ca2 a b (ConstraintAutomata.T ca1 a) (ConstraintAutomata.T ca2 b) [])
+                                     (computeTransitivity ca1 ca2 t setPairsFull)
+                      end
+  end.*)
+
+   Definition isBisim (setPairs : set (state * state)) :=
+    isSymmetric setPairs.
+
+  Definition bisimulation (ca1: constraintAutomata) (ca2: constraintAutomata) :=
+    isBisim (bisimulationAux ca1 ca2).
+
+
+  (* We calculate the partition Q / R *)
+  Fixpoint mountSubsetFromPairs (pairStates : state) (setPairs : set (state * state)) :=
+    match setPairs with
+    | [] => [pairStates]
+    | a::t => if (fst(a) == pairStates) then set_add equiv_dec (snd(a)) (mountSubsetFromPairs pairStates t)
+              else mountSubsetFromPairs pairStates t
+    end.
+
+  Fixpoint getQrelR (setRel : set (state * state)) :=
+    match setRel with
+    | [] => []
+    | a::t =>  set_add equiv_dec (mountSubsetFromPairs (fst(a)) (setRel)) (getQrelR t)
+    end.
+
+
+  (* We define the Notation 3.8, DC_A(q,N,P) as Baier et al. define for bisimulation as dcsOfState *)
+
+  Fixpoint getReachedDcs (t: set (set name * DC name data * state)) (setStates: set state) :=
+    match t with
+    | [] => []
+    | a::t => if set_mem equiv_dec (snd(a)) (setStates)
+              then (snd(fst(a)))::(getReachedDcs t setStates)
+              else (getReachedDcs t setStates)
+    end.
+
+  Fixpoint orDcs (dc : DC name data) :=
+    match dc with
+    | andDc a b => ConstraintAutomata.orDc (ConstraintAutomata.negDc (orDcs a)) (ConstraintAutomata.negDc(orDcs b))
+    | _ => dc
+    end.
+
+  (* Then we build the disjunction of all dcs of a single transition that reaches a state in P *)
+  Fixpoint disjunctionOfDcs (setDcs : set(DC name data))  :=
+    match setDcs with
+    | [] => ConstraintAutomata.negDc(ConstraintAutomata.tDc name data)
+    | a::t => match a with
+              | andDc x y => (ConstraintAutomata.orDc (orDcs a) (disjunctionOfDcs t)) 
+              | _ => (ConstraintAutomata.orDc (a) (disjunctionOfDcs t))
+              end
+    end.
+
+   Definition dcsOfState (ca: constraintAutomata) (q: state) (portNames : set name) (P: set state) :=
+    disjunctionOfDcs((getReachedDcs (getTransition (portNames) (ConstraintAutomata.T ca q))) (P)).
+
+  (* Equivalence for DCs. Requires that an equality relation to be defined for functions data -> data *)
+  Context `{EqDec (data -> data) eq}.
+  
+  Instance dc_eqDec `(EqDec name eq) `(EqDec data eq)  : EqDec (DC name data) eq :=
+    { equiv_dec := fix rec dc1 dc2 :=
+      match dc1,dc2 with
+       | tDc _ _, tDc _ _ => in_left
+       | dc a b, dc c d => if a == c then if b == d then in_left else in_right else in_right
+       | eqDc _ a b, eqDc _ c d => if a == c then if b == d then in_left else in_right else in_right
+       | andDc a b, andDc c d => if rec a c then if rec b d then in_left else in_right else in_right
+       | orDc a b, orDc c d => if rec a c then if rec b d then in_left else in_right else in_right
+       | negDc a, negDc b => if rec a b then in_left else in_right
+       | trDc f a b, trDc g c d => if f == g then if a == c then if b == d then in_left else in_right else in_right else in_right
+       | _, _ => in_right
+      end
+    }.
+    Proof. 
+    all : congruence.
+    Defined.
+
+  (* After reconstructing a DC as Notation 3.8 from a set of possible data constraints of transitions q -> P *)
+  (* We need to evaluate whether they are equivalent or not                                                  *)
+  Fixpoint dismantleDc (dc: DC name data) :=
+    match dc with
+    | tDc _ _ => [tDc _ _]
+    | eqDc _ a b => [eqDc _ a b]
+    | dc a b => [dc]
+    | negDc a => [negDc a]
+    | trDc f a b => [trDc f a b]
+    | orDc a b | andDc a b => set_union equiv_dec (dismantleDc a) (dismantleDc b)
+    end.
+
+  (* We search for conditions !A \/ A or \top in a single DC, which makes it always true *)
+
+  Fixpoint existsComplementOrTrue (setDc : set (DC name data)) :=
+    match setDc with
+    | [] => false
+    | a::t => match a with
+              | tDc _ _ => true
+              | _ => if (set_mem equiv_dec (negDc(a)) (setDc)) then true else (existsComplementOrTrue t)
+              end
+    end.
+
+  Lemma existsComplementOrTrueSound  : forall setDc,
+    existsComplementOrTrue setDc = true -> In (tDc _ _) setDc \/ (exists a, In (a) (setDc) /\ In (negDc(a)) (setDc)).
+  Proof.
+  - intros. induction setDc. inversion H3. simpl in H3. destruct a. left. simpl;auto.
+  + destruct equiv_dec in H3. inversion e. destruct set_mem eqn:ha in H3. apply set_mem_correct1 in ha. unfold set_In in ha. 
+    right. exists (dc n d). split. simpl;auto. simpl. right. exact ha. apply IHsetDc in H3.
+    destruct H3. left. simpl;auto. destruct H3. destruct H3. right. exists x. split.
+    simpl. right. assumption. simpl. right. assumption. 
+  + destruct equiv_dec in H3. inversion e. destruct set_mem eqn:ha in H3. apply set_mem_correct1 in ha. unfold set_In in ha. 
+    right. exists (eqDc data n n0). split. simpl;auto. simpl. right. exact ha. apply IHsetDc in H3.
+    destruct H3. left. simpl;auto. destruct H3. destruct H3. right. exists x. split.
+    simpl. right. assumption. simpl. right. assumption. 
+  + destruct equiv_dec in H3. inversion e. destruct set_mem eqn:ha in H3. apply set_mem_correct1 in ha. unfold set_In in ha. 
+    right. exists (a1 @ a2). split. simpl;auto. simpl. right. exact ha. apply IHsetDc in H3.
+    destruct H3. left. simpl;auto. destruct H3. destruct H3. right. exists x. split.
+    simpl. right. assumption. simpl. right. assumption. 
+  + destruct equiv_dec in H3. inversion e. destruct set_mem eqn:ha in H3. apply set_mem_correct1 in ha. unfold set_In in ha. 
+    right. exists (a1 $ a2) . split. simpl;auto. simpl. right. exact ha. apply IHsetDc in H3.
+    destruct H3. left. simpl;auto. destruct H3. destruct H3. right. exists x. split.
+    simpl. right. assumption. simpl. right. assumption. 
+  + destruct equiv_dec in H3. inversion e. destruct set_mem eqn:ha in H3. apply set_mem_correct1 in ha. unfold set_In in ha. 
+    right. exists (trDc d n n0). split. simpl;auto. simpl. right. exact ha. apply IHsetDc in H3.
+    destruct H3. left. simpl;auto. destruct H3. destruct H3. right. exists x. split.
+    simpl. right. assumption. simpl. right. assumption. 
+  + destruct equiv_dec in H3. inversion e.
+    right. exists (negDc a). split. simpl;auto. simpl. left. reflexivity. destruct set_mem eqn:ha in H3. apply set_mem_correct1 in ha. unfold set_In in ha. 
+    right. exists (negDc a). split. simpl;auto. simpl. right. exact ha. apply IHsetDc in H3.
+    destruct H3. left. simpl;auto. destruct H3. destruct H3. right. exists x. split.
+    simpl. right. assumption. simpl. right. assumption. 
+    Qed.
+    
+
+  Definition areEquivalentAux (dc1 : set (DC name data)) (dc2: set (DC name data)) :=
+    set_eq ((dc1)) ((dc2)) || 
+      ((existsComplementOrTrue dc1) && (existsComplementOrTrue dc2)).
+
+  (* We define equivalence of DCs as defined by Notation 3.8 (aforementioned) *)
+  Fixpoint areEquivalent (dc1 : DC name data) (dc2: DC name data) :=
+    areEquivalentAux (dismantleDc dc1) (dismantleDc dc2).
+
+  (*We define the powerset's construction, in order to verify all possible port names' labels for transitions *)
+  Fixpoint powerset (s: set name) :=
+    match s with 
+    | [] => []
+    | a::t => concat (map (fun f => [a::f;f]) (powerset t))
+    end.
+
+  (* The comparison of dcsOfState for all port names of both automata *)
+  Fixpoint compareDcBisimPortName (ca1: constraintAutomata) (ca2: constraintAutomata) (q1: state)
+  (q2: state) (P: set state) (setNames: set (set name)) :=
+    match setNames with
+    | [] => true
+    | a::t => areEquivalent((dcsOfState (ca1) (q1) a P)) ((dcsOfState (ca2) (q2) a P)) && 
+              (compareDcBisimPortName ca1 ca2 q1 q2 P t)
+    end.
+
+  (* Now we want to know if compareDcBisimPortName holds for every P \in Q / R as elements of the bisimulation relation *)
+  Fixpoint compareDcBisimPartition (ca1: constraintAutomata) (ca2: constraintAutomata) (q1: state)
+  (q2: state) (setNames: set (set name)) (qMinusR : set (set state)):=
+    match qMinusR with
+    | [] => true
+    | a::t => (compareDcBisimPortName ca1 ca2 q1 q2 a setNames) && (compareDcBisimPartition ca1 ca2 q1 q2 setNames t)
+    end.
+
+  (* We need to check if the above condition holds for every pair of states (q1,q2) \in R as the bisim. relation *)
+  Fixpoint compareDcBisimStates (ca1: constraintAutomata) (ca2: constraintAutomata) 
+  (setNames: set (set name)) (qMinusR : set (set state)) (pairStates : set (state * state)) :=
+    match pairStates with
+    | [] => true
+    | a::t =>  (compareDcBisimPartition ca1 ca2 (fst(a)) (snd(a)) setNames qMinusR) &&
+               (compareDcBisimStates ca1 ca2 setNames qMinusR t)
+    end.
+
+  (* We have to ensure that all states of both CA have been comprehended by the obtained bisimulation relation *)
+
+  Fixpoint statesA1InSetPairStates (setPairStates: set (state * state)) : set state:=
+    match setPairStates with
+    | [] => []
+    | a::t => set_add equiv_dec (fst(a)) (statesA1InSetPairStates t)
+    end.
+
+  Fixpoint statesA2InSetPairStates (setPairStates: set (state * state)) : set state:=
+    match setPairStates with
+    | [] => []
+    | a::t => set_add equiv_dec (snd(a)) (statesA2InSetPairStates t)
+    end.
+
+  Definition containsAllStatesOfBothCa (setQ1 : set state) (setQ2 : set state) (setBisim : set (state * state)) :=
+    (s1_in_s2 (setQ1) (statesA1InSetPairStates setBisim)) && (s1_in_s2 (setQ2) (statesA2InSetPairStates setBisim)).
+  
+  Definition checkBisimilarity (ca1: constraintAutomata) (ca2: constraintAutomata) (bisimRelation : set (state * state)) :=
+    if (set_eq (ConstraintAutomata.N ca1) (ConstraintAutomata.N ca2)) && (negb(equiv_decb (bisimRelation) ([]))) then  
+    compareDcBisimStates ca1 ca2 (powerset (ConstraintAutomata.N ca1)) (getQrelR (bisimRelation)) (bisimRelation)  &&
+    containsAllStatesOfBothCa (ConstraintAutomata.Q0 ca1) (ConstraintAutomata.Q0 ca2) (bisimRelation)(*(containsSymmetric (bisimRelation) (bisimRelation))*)
+    else false.
+    
+  Definition areBisimilar (ca1: constraintAutomata) (ca2: constraintAutomata) :=
+    checkBisimilarity ca1 ca2 (bisimulation ca1 ca2).
+ 
   End ConstraintAutomata.
-End ConstraintAutomata.
+End ConstraintAutomata. 
 
 Module ProductAutomata.
   Section ProductAutomata.
     Variable state name data state2: Set.
-    Context `{EqDec name eq} `{EqDec state eq} `{EqDec state2 eq} `{EqDec (option data) eq}.
+    Context `{EqDec name eq} `{EqDec state eq} `{EqDec state2 eq} `{EqDec (data) eq}.
 
     Definition constraintAutomata  := ConstraintAutomata.constraintAutomata state name data.
     Definition constraintAutomata2 := ConstraintAutomata.constraintAutomata state2 name data.
     Definition DC := ConstraintAutomata.DC name data.
 
-    Definition resultingStatesSet (a1:ConstraintAutomata.constraintAutomata state name data) (a2:ConstraintAutomata.constraintAutomata state2 name data) :=
+    Definition statesSet (a1:ConstraintAutomata.constraintAutomata state name data) (a2:ConstraintAutomata.constraintAutomata state2 name data) :=
       list_prod (ConstraintAutomata.Q a1) (ConstraintAutomata.Q a2).
-    Check resultingStatesSet.
 
-    Lemma resultingStatesSetSound :forall a1,forall a2, forall a, forall b,
-      In (a,b) (resultingStatesSet a1 a2) <-> In a (ConstraintAutomata.Q a1) /\ In b (ConstraintAutomata.Q a2).
+    Lemma statesSetSound :forall a1,forall a2, forall a, forall b,
+      In (a,b) (statesSet a1 a2) <-> In a (ConstraintAutomata.Q a1) /\ In b (ConstraintAutomata.Q a2).
     Proof.
     intros. apply in_prod_iff. 
     Defined.
 
-    Definition resultingNameSet (a1:ConstraintAutomata.constraintAutomata state name data) (a2:ConstraintAutomata.constraintAutomata state2 name data) :=
+    Definition nameSet (a1:ConstraintAutomata.constraintAutomata state name data) (a2:ConstraintAutomata.constraintAutomata state2 name data) :=
       set_union equiv_dec (ConstraintAutomata.N a1) (ConstraintAutomata.N a2).
     
-    Lemma resultingNameSetSound : forall a1, forall a2, forall a,
-      In a (resultingNameSet a1 a2) <-> In a (ConstraintAutomata.N a1) \/ In a (ConstraintAutomata.N a2).
+    Lemma nameSetSound : forall a1, forall a2, forall a,
+      In a (nameSet a1 a2) <-> In a (ConstraintAutomata.N a1) \/ In a (ConstraintAutomata.N a2).
     Proof.
     intros. apply set_union_iff.
     Defined.
 
-    Definition resultingInitialStatesSet (a1: constraintAutomata) (a2: constraintAutomata2) :=
+    Definition initialStates (a1: constraintAutomata) (a2: constraintAutomata2) :=
       list_prod (ConstraintAutomata.Q0 a1) (ConstraintAutomata.Q0 a2).
 
-    Lemma resultingInitialStatesSetSound : forall a1, forall a2, forall a, forall b,
-      In (a,b) (resultingInitialStatesSet a1 a2) <-> In a (ConstraintAutomata.Q0 a1) /\ In b (ConstraintAutomata.Q0 a2).
+    Lemma initialStatesSound : forall a1, forall a2, forall a, forall b,
+      In (a,b) (initialStates a1 a2) <-> In a (ConstraintAutomata.Q0 a1) /\ In b (ConstraintAutomata.Q0 a2).
     Proof.
     intros. apply in_prod_iff. 
     Defined.
 
   
-    Definition evaluateConditionsFirstRule (t1 : ( set(name) * DC * set(state))) (t2 : (set(name) * DC * set(state2)))
+    Definition condR1 (t1 : ( set(name) * DC * state)) (t2 : (set(name) * DC * state2))
       (names1 : set name) (names2: set name) :=
-      if set_eq (set_inter equiv_dec (names2) (fst(fst(t1)))) (set_inter equiv_dec (names1) (fst(fst(t2)))) then true else false.
+      set_eq (set_inter equiv_dec (names2) (fst(fst(t1)))) (set_inter equiv_dec (names1) (fst(fst(t2)))).
 
-    Lemma evaluateConditionsFirstRuleSound : forall t1, forall t2, forall names1, forall names2,
-    evaluateConditionsFirstRule t1 t2 names1 names2 = true <-> 
+    Lemma condR1Sound : forall t1, forall t2, forall names1, forall names2,
+    condR1 t1 t2 names1 names2 = true <-> 
     set_eq (set_inter equiv_dec (names2) (fst(fst(t1)))) (set_inter equiv_dec (names1) (fst(fst(t2)))) = true.
     Proof. 
     split. 
-    - intros. unfold evaluateConditionsFirstRule in H2. case_eq (set_eq (set_inter equiv_dec names2 (fst (fst t1)))
+    - intros. unfold condR1 in H2. case_eq (set_eq (set_inter equiv_dec names2 (fst (fst t1)))
          (set_inter equiv_dec names1 (fst (fst t2)))).
     + intros. reflexivity.
-    + intros. unfold evaluateConditionsFirstRule in H3. rewrite H4 in H3. discriminate.
-    - intros. unfold evaluateConditionsFirstRule. rewrite H3. reflexivity.
+    + intros. unfold condR1 in H3. rewrite H4 in H3. discriminate.
+    - intros. unfold condR1. rewrite H3. reflexivity.
     Defined.
 
-    Fixpoint buildResultingTransitionFromStatesRule1 (p1: state) (p2: set state2) :=
-      match p2 with
-      | [] => []
-      | a::t => (p1,a)::
-                buildResultingTransitionFromStatesRule1 p1 t
-      end.
-    Lemma buildResultingTransitionFromStatesRule1Sound : forall p1, forall p2, 
-      buildResultingTransitionFromStatesRule1 p1 p2 <> [] <-> p2 <> [].
-    Proof.
-    split.
-    - intros. destruct p2.
-    + simpl in H3. congruence.
-    + discriminate.
-    - intros. destruct p2.
-    + congruence.
-    + discriminate.
-    Defined.
-    Check buildResultingTransitionFromStatesRule1.
-
-    Fixpoint buildResultingTransitionFromStatesBothTransitionsRule1 (p1: set state) (p2: set state2) :=
-      match p1 with
-      | [] => []
-      | a::t => buildResultingTransitionFromStatesRule1 a p2++
-                buildResultingTransitionFromStatesBothTransitionsRule1 t p2
-      end.
-    Check buildResultingTransitionFromStatesBothTransitionsRule1.
-
-    Definition buildResultingTransitionFromSingleStateRule1 (Q1: state) (Q2: state2)
-      (transition1: (set (name) * DC * (set(state)))) 
-      (transition2: (set (name) * DC * (set(state2)))) 
-      (names1 : set name) (names2: set name) :  (set (state * state2 * ((set name * DC) * set (state * state2)))) :=
-      if (evaluateConditionsFirstRule (transition1) (transition2) (names1) (names2)) == true then
+    Definition singleTransitionR1 (Q1: state) (Q2: state2)
+      (transition1: (set (name) * DC * (state))) 
+      (transition2: (set (name) * DC * (state2))) 
+      (names1 : set name) (names2: set name) :  (set (state * state2 * ((set name * DC) * (state * state2)))) :=
+        if (condR1 (transition1) (transition2) (names1) (names2)) then
                   [((Q1,Q2),(((set_union equiv_dec (fst(fst(transition1))) (fst(fst(transition2)))),ConstraintAutomata.andDc (snd(fst(transition1))) 
-                            (snd(fst(transition2)))),(buildResultingTransitionFromStatesBothTransitionsRule1(snd(transition1)) (snd(transition2)))))]
-                else [].
+                            (snd(fst(transition2)))),(snd(transition1) , (snd(transition2)))))]
+        else [].
 
-    Lemma buildResultingTransitionFromSingleStateRule1Sound : forall Q1, forall Q2, forall transition1, 
-    forall transition2, forall names1, forall names2, buildResultingTransitionFromSingleStateRule1 Q1 Q2 transition1 transition2
-    names1 names2 <> [] <-> (evaluateConditionsFirstRule (transition1) (transition2) (names1) (names2)) = true.
+    Lemma singleTransitionR1Sound : forall Q1, forall Q2, forall transition1, 
+    forall transition2, forall names1, forall names2, singleTransitionR1 Q1 Q2 transition1 transition2
+    names1 names2 <> [] <-> (condR1 (transition1) (transition2) (names1) (names2)) = true.
     Proof.
     split.
-    - intros. unfold buildResultingTransitionFromSingleStateRule1 in H3. destruct equiv_dec. inversion e. reflexivity. congruence.
-    - intros. unfold buildResultingTransitionFromSingleStateRule1. rewrite H3. simpl. discriminate.
+    - intros. unfold singleTransitionR1 in H3. 
+      case_eq (condR1 (transition1) (transition2) (names1) (names2)). reflexivity. 
+      intros. rewrite H4 in H3. congruence.
+    - intros. unfold singleTransitionR1. rewrite H3. discriminate.
     Defined.
 
-    Check buildResultingTransitionFromSingleStateRule1.
-
-    Fixpoint buildTransitionFromMoreTransitionsRule1 (Q1: state) (Q2: state2)
-      (transition1: (set (name) * DC * (set(state)))) 
-      (transition2: set (set (name) * DC * (set(state2)))) 
+    Fixpoint moreTransitionsR1 (Q1: state) (Q2: state2)
+      (transition1: (set (name) * DC * (state))) 
+      (transition2: set (set (name) * DC * (state2))) 
       (names1 : set name) (names2: set name) :=
       match transition2 with
       | [] => []
-      | a::t => (buildResultingTransitionFromSingleStateRule1 Q1 Q2 transition1 a names1 names2)++
-                (buildTransitionFromMoreTransitionsRule1 Q1 Q2 transition1 t names1 names2)
+      | a::t => (singleTransitionR1 Q1 Q2 transition1 a names1 names2)++
+                (moreTransitionsR1 Q1 Q2 transition1 t names1 names2)
       end.
-    Check buildTransitionFromMoreTransitionsRule1.
 
-    Fixpoint buildTransitionFromMoreAllTransitionsSingleState (Q1: state) (Q2: state2)
-      (transition1: set (set (name) * DC * (set(state)))) 
-      (transition2: set (set (name) * DC * (set(state2)))) 
+    Fixpoint transitionsForOneStateR1 (Q1: state) (Q2: state2)
+      (transition1: set (set (name) * DC * (state))) 
+      (transition2: set (set (name) * DC * (state2))) 
       (names1 : set name) (names2: set name) :=
       match transition1 with
       | [] => []
-      | a::t => (buildTransitionFromMoreTransitionsRule1 Q1 Q2 a transition2 names1 names2)++
-                (buildTransitionFromMoreAllTransitionsSingleState Q1 Q2 t transition2 names1 names2)
+      | a::t => (moreTransitionsR1 Q1 Q2 a transition2 names1 names2)++
+                (transitionsForOneStateR1 Q1 Q2 t transition2 names1 names2)
       end.
 
-    Fixpoint iterateOverStatesBuildingTransitionsOne (Q1: state) (Q2: set state2)
-      (transition1: state -> set (set (name) * DC * (set(state)))) 
-      (transition2: state2 -> set (set (name) * DC * (set(state2)))) 
+    Fixpoint iterateOverA2R1 (Q1: state) (Q2: set state2)
+      (transition1: state -> set (set (name) * DC * (state))) 
+      (transition2: state2 -> set (set (name) * DC * (state2))) 
       (names1 : set name) (names2: set name) :=
       match Q2 with
       | [] => []
-      | a::t => (buildTransitionFromMoreAllTransitionsSingleState Q1 a (transition1 Q1) (transition2 a) names1 names2)++
-                (iterateOverStatesBuildingTransitionsOne Q1 t transition1 transition2 names1 names2)
+      | a::t => (transitionsForOneStateR1 Q1 a (transition1 Q1) (transition2 a) names1 names2)++
+                (iterateOverA2R1 Q1 t transition1 transition2 names1 names2)
       end.
 
-    Fixpoint buildAllTransitionsRule1 (Q1: set state) (Q2: set state2)
-      (transition1: state -> set (set (name) * DC * (set(state)))) 
-      (transition2: state2 -> set (set (name) * DC * (set(state2)))) 
+    Fixpoint allTransitionsR1 (Q1: set state) (Q2: set state2)
+      (transition1: state -> set (set (name) * DC * (state))) 
+      (transition2: state2 -> set (set (name) * DC * (state2))) 
       (names1 : set name) (names2: set name) :=
       match Q1 with
       | [] => []
-      | a::t => (iterateOverStatesBuildingTransitionsOne a Q2 transition1 transition2 names1 names2)++
-                (buildAllTransitionsRule1 t Q2 transition1 transition2 names1 names2)
+      | a::t => (iterateOverA2R1 a Q2 transition1 transition2 names1 names2)++
+                (allTransitionsR1 t Q2 transition1 transition2 names1 names2)
     end. 
-    Definition transitionsRule1 (a1: constraintAutomata) (a2: constraintAutomata2) := 
-      buildAllTransitionsRule1 (ConstraintAutomata.Q a1) (ConstraintAutomata.Q a2) 
-                               (ConstraintAutomata.T a1) (ConstraintAutomata.T a2) 
-                               (ConstraintAutomata.N a1) (ConstraintAutomata.N a2).
-    Check transitionsRule1.
 
-    Definition intersectionNAndNames (tr: set (name) * DC * set(state)) (names2: set name) :=
+
+    Definition transitionsRule1 (a1: constraintAutomata) (a2: constraintAutomata2) := 
+      allTransitionsR1 (ConstraintAutomata.Q a1) (ConstraintAutomata.Q a2) 
+                       (ConstraintAutomata.T a1) (ConstraintAutomata.T a2) 
+                       (ConstraintAutomata.N a1) (ConstraintAutomata.N a2).
+
+    Definition condR2 (tr: set (name) * DC * state) (names2: set name) :=
       if (set_inter equiv_dec (fst(fst(tr))) names2) == nil then true else false.
 
-    Lemma intersectionNAndNamesSound : forall tr, forall names2, intersectionNAndNames tr names2 = true <->
+    Lemma condR2Sound : forall tr, forall names2, condR2 tr names2 = true <->
       set_inter equiv_dec (fst(fst(tr))) names2 = nil.
     Proof.
     split.
-    - intros. unfold intersectionNAndNames in H3. destruct equiv_dec in H3. inversion e. reflexivity.
+    - intros. unfold condR2 in H3. destruct equiv_dec in H3. inversion e. reflexivity.
       inversion H3.
-    - intros. unfold intersectionNAndNames. rewrite H3. reflexivity.
+    - intros. unfold condR2. rewrite H3. reflexivity.
     Defined.
 
-    Fixpoint iterateOverOutboundStatesRule2  (p1: set state) (q2: state2) :=
-      match p1 with
-      | [] => []
-      | a::t => set_add equiv_dec ((a,q2))(iterateOverOutboundStatesRule2 t q2)
-      end.
-    Check iterateOverOutboundStatesRule2.
-
-    Fixpoint iterateOverOutboundStatesRule3 (q1: state) (p2: set state2) :=
-      match p2 with
-      | [] => []
-      | a::t => set_add equiv_dec ((q1,a))(iterateOverOutboundStatesRule3 q1 t)
-      end.
-    Check iterateOverOutboundStatesRule3.
-
-    Fixpoint createSingleTransition (q1:state) (transition : (set (name) * DC * (set(state)))) (a2States : set state2) (a2Names: set name)   
-    : set (state * state2 * ((set name * DC) * set (state * state2))) :=
+    Fixpoint singleTransitionR2 (q1:state) (transition : (set (name) * DC * (state))) (a2States : set state2) (a2Names: set name)   
+    : set (state * state2 * ((set name * DC) * (state * state2))) :=
     match a2States with
     | [] => []
-    | q2::t => if (intersectionNAndNames (transition) (a2Names) == true) then 
-                 ((q1,q2),((fst(transition)), (iterateOverOutboundStatesRule2 (snd(transition)) (q2))))::createSingleTransition q1 transition t a2Names
-                else createSingleTransition q1 transition t a2Names
+    | q2::t => if (condR2 (transition) (a2Names)) then 
+                 ((q1,q2),((fst(transition)), ((snd(transition)), (q2))))::singleTransitionR2 q1 transition t a2Names
+                else singleTransitionR2 q1 transition t a2Names
     end.
-    Check createSingleTransition.
 
-    Lemma createSingleTransitionSound : forall q1, forall transition, forall a2States, forall a2Names, 
-      createSingleTransition q1 transition a2States a2Names <> [] <-> intersectionNAndNames (transition) (a2Names) = true /\ a2States <> [].
+    Lemma singleTransitionR2Sound : forall q1, forall transition, forall a2States, forall a2Names, 
+      singleTransitionR2 q1 transition a2States a2Names <> [] <-> condR2 (transition) (a2Names) = true /\ a2States <> [].
     Proof.
     split.
-    - intros. induction a2States. unfold createSingleTransition in H3. congruence.
-      simpl in H3. case_eq (intersectionNAndNames transition a2Names). intros. split. reflexivity. congruence.
+    - intros. induction a2States. unfold singleTransitionR2 in H3. congruence.
+      simpl in H3. case_eq (condR2 transition a2Names). intros. split. reflexivity. congruence.
       intros. rewrite H4 in H3. simpl in H3. apply IHa2States in H3. destruct H3. congruence.
-    - intros. induction a2States. unfold createSingleTransition. destruct H3. congruence.
-      simpl. destruct equiv_dec. discriminate. apply IHa2States. destruct H3. congruence.
+    - intros. induction a2States. unfold singleTransitionR2. destruct H3. congruence.
+      simpl. case_eq (condR2 transition a2Names). discriminate. intros. destruct H3. congruence.
     Defined.
      
-    Definition createTransitionRule2 (q1:state) : set (set (name) * DC * (set(state))) -> 
+    Definition transitionR2 (q1:state) : set (set (name) * DC * (state)) -> 
       set state2 -> set name 
-      -> set (state * state2 * ((set name * DC) * set (state * state2))) :=
+      -> set (state * state2 * ((set name * DC) * (state * state2))) :=
       fix rec transitions q2 names2 :=
         match transitions with
         | [] => [] 
-        | a::t =>  (createSingleTransition q1 a q2 names2)++(rec t q2 names2)
+        | a::t =>  (singleTransitionR2 q1 a q2 names2)++(rec t q2 names2)
         end.
-    Check createTransitionRule2.
 
-    Fixpoint createTransitionRule2AllStates (Q1: set state) (transitions: state -> set (set (name) * DC * (set(state)))) 
+    Fixpoint allTransitionsR2 (Q1: set state) (transitions: state -> set (set (name) * DC * (state))) 
       (names2: set name) (a2States : set state2) := 
       match Q1 with
       | [] => []
-      | a::t => (createTransitionRule2 a (transitions(a)) a2States names2)++(createTransitionRule2AllStates t transitions names2 a2States)
+      | a::t => (transitionR2 a (transitions(a)) a2States names2)++(allTransitionsR2 t transitions names2 a2States)
       end.
-    Check createTransitionRule2.
 
     Definition transitionsRule2 (a1: constraintAutomata) (a2 : constraintAutomata2)  :=
-      (createTransitionRule2AllStates (ConstraintAutomata.Q a1) (ConstraintAutomata.T a1) 
+      (allTransitionsR2 (ConstraintAutomata.Q a1) (ConstraintAutomata.T a1) 
                                       (ConstraintAutomata.N a2) (ConstraintAutomata.Q a2)).
-    Check transitionsRule2.
 
-    Definition intersectionNAndNames2 (tr: set (name) * DC * set(state2)) (names1: set name) :=
+    Definition condR3 (tr: set (name) * DC * state2) (names1: set name) :=
       if (set_inter equiv_dec (fst(fst(tr))) names1) == nil then true else false.
 
-    Lemma intersectionNAndName2Sound : forall tr, forall names1, intersectionNAndNames2 tr names1 = true <->
+    Lemma condR3Sound : forall tr, forall names1, condR3 tr names1 = true <->
       set_inter equiv_dec (fst(fst(tr))) names1 = nil.
     Proof.
     split.
-    - intros. unfold intersectionNAndNames2 in H3. destruct equiv_dec in H3. inversion e. reflexivity.
+    - intros. unfold condR3 in H3. destruct equiv_dec in H3. inversion e. reflexivity.
       inversion H3.
-    - intros. unfold intersectionNAndNames2. rewrite H3. reflexivity.
+    - intros. unfold condR3. rewrite H3. reflexivity.
     Defined.
 
-    Fixpoint createSingleTransitionRule3 (q2:state2) (transition : (set (name) * DC * (set(state2)))) (a2States : set state) (a1Names: set name)   
-    : set (state * state2 * ((set name * DC) * set (state * state2))) :=
+    Fixpoint singleTransitionR3 (q2:state2) (transition : (set (name) * DC * (state2))) (a2States : set state) (a1Names: set name)   
+    : set (state * state2 * ((set name * DC) * (state * state2))) :=
     match a2States with
     | [] => []
-    | q1::t => if (intersectionNAndNames2 (transition) (a1Names) == true) then 
-                 ((q1,q2),((fst(transition)), (iterateOverOutboundStatesRule3 (q1) (snd(transition)))))::createSingleTransitionRule3 q2 transition t a1Names
-                else createSingleTransitionRule3 q2 transition t a1Names
+    | q1::t => if (condR3 (transition) (a1Names)) then 
+                 ((q1,q2),((fst(transition)), ((q1) , (snd(transition)))))::singleTransitionR3 q2 transition t a1Names
+                else singleTransitionR3 q2 transition t a1Names
     end.
 
-    Lemma createSingleTransitionRule3Sound : forall q2, forall transition, forall a1States, forall a1Names,
-    createSingleTransitionRule3 q2 transition a1States a1Names <> [] <-> 
-    intersectionNAndNames2 (transition) (a1Names) = true /\ a1States <> [].
+    Lemma singleTransitionR3Sound : forall q2, forall transition, forall a1States, forall a1Names,
+    singleTransitionR3 q2 transition a1States a1Names <> [] <-> 
+    condR3 (transition) (a1Names) = true /\ a1States <> [].
     Proof.
     split. 
     - intros. induction a1States. simpl in H3. congruence.
-    simpl in H3. destruct equiv_dec in H3. inversion e. split. reflexivity. discriminate.
-    apply IHa1States in H3. destruct H3. congruence.
+    simpl in H3. case_eq (condR3 (transition) (a1Names)). split. reflexivity. discriminate.
+    intros. rewrite H4 in H3. apply IHa1States in H3. destruct H3. congruence.
     - intros. induction a1States. destruct H3. congruence.
-    simpl. destruct equiv_dec. discriminate.
+    simpl. case_eq (condR3 (transition) (a1Names)). discriminate.
     destruct H3. congruence.
     Defined.
   
-    Definition createTransitionRule3 (q2:state2) : set (set (name) * DC * (set(state2))) -> 
+    Definition transitionR3 (q2:state2) : set (set (name) * DC * (state2)) -> 
       set state -> set name  
-      -> set (state * state2 * ((set name * DC) * set (state * state2))) :=
+      -> set (state * state2 * ((set name * DC) * (state * state2))) :=
       fix rec transitions q1 names1 :=
         match transitions with
         | [] => [] 
-        | a::t =>  (createSingleTransitionRule3 q2 a q1 names1)++(rec t q1 names1)
+        | a::t =>  (singleTransitionR3 q2 a q1 names1)++(rec t q1 names1)
         end.
-    Check createTransitionRule3.
 
-    Fixpoint createTransitionRule3AllStates (Q2: set state2) (transitions: state2 -> set (set (name) * DC * (set(state2)))) 
+    Fixpoint allTransitionsR3 (Q2: set state2) (transitions: state2 -> set (set (name) * DC * (state2))) 
       (names1: set name) (a1States : set state) := 
       match Q2 with
       | [] => []
-      | a::t => (createTransitionRule3 a (transitions(a)) a1States names1)++(createTransitionRule3AllStates t transitions names1 a1States)
+      | a::t => (transitionR3 a (transitions(a)) a1States names1)++(allTransitionsR3 t transitions names1 a1States)
       end.
 
     Definition transitionsRule3 (a1: constraintAutomata) (a2 : constraintAutomata2)  :=
-      (createTransitionRule3AllStates (ConstraintAutomata.Q a2) (ConstraintAutomata.T a2) 
-                                      (ConstraintAutomata.N a1) (ConstraintAutomata.Q a1)).
-    Check transitionsRule3. 
+      (allTransitionsR3 (ConstraintAutomata.Q a2) (ConstraintAutomata.T a2) 
+                       (ConstraintAutomata.N a1) (ConstraintAutomata.Q a1)).
 
     Definition buildTransitionRuleProductAutomaton (a1: constraintAutomata) (a2: constraintAutomata2) :=
       (transitionsRule1 a1 a2)++(transitionsRule2 a1 a2)++(transitionsRule3 a1 a2).
-    Check buildTransitionRuleProductAutomaton.
-
-  
-    Variable a1 : (constraintAutomata).
-    Variable a2 : (constraintAutomata2).
 
     Fixpoint recoverResultingStatesPA (st: (state * state2)) 
-      (t:set (state * state2 * ((set name * DC) * set (state * state2))))(*: set ((state * state)) *):=
+      (t:set (state * state2 * ((set name * DC) * (state * state2)))) :=
       match t with
       | [] => []
       | a::tx => if st == fst((a)) then (snd((a))::recoverResultingStatesPA st tx)
                  else recoverResultingStatesPA st tx
       end.
-    Check recoverResultingStatesPA.
 
     Lemma recoverResultingStatesPASound : forall st, forall t, recoverResultingStatesPA st t <> [] <->
       exists a, In a t /\ st = fst(a).
@@ -866,11 +1089,11 @@ Module ProductAutomata.
       rewrite <- H3 in H4. congruence. exists x. split. exact H3. exact H4.
     Defined.
 
-    Definition transitionPA (s: (state * state2)) :=
+    Definition transitionPA (a1: constraintAutomata) (a2: constraintAutomata2) (s: (state * state2)) :=
       recoverResultingStatesPA s (buildTransitionRuleProductAutomaton a1 a2). 
 
-    Definition buildPA := ConstraintAutomata.CA 
-      (resultingStatesSet a1 a2) (resultingNameSet a1 a2) (transitionPA) (resultingInitialStatesSet a1 a2). 
+    Definition buildPA (a1: constraintAutomata) (a2:constraintAutomata2) := 
+      ConstraintAutomata.CA (statesSet a1 a2) (nameSet a1 a2) (transitionPA a1 a2) (initialStates a1 a2).
 
   End ProductAutomata.
 End ProductAutomata.
